在 $x=0$ 处判断：

对于 $x<0$，有 $f(x)=-(x^3-x)g(x)$，对于 $x>0$，有 $f(x)=(x^3-x)g(x)$。因为 $g(x)$ 是连续函数，所以只需要考虑 $f(x)$ 的可导性。

当 $x>0$ 时，有 $f'(x)=(3x^2-1)g(x)+(x^3-x)g'(x)$，因为 $g(x)$ 连续，所以 $(3x^2-1)g(x)$ 可导，只需考虑 $(x^3-x)g'(x)$ 的可导性。因为 $x>0$，所以 $x^3-x>0$，所以 $f(x)$ 可导。

当 $x<0$ 时，有 $f'(x)=-(3x^2-1)g(x)-(x^3-x)g'(x)$，同理可得 $f(x)$ 可导。

综上，$f(x)$ 在 $x=0$ 处可导。

在 $x=1$ 处判断：

当 $x>1$ 时，有 $f(x)=(x^3-x)g(x)$，当 $x<1$ 时，有 $f(x)=-(x^3-x)g(x)$。因为 $g(x)$ 是连续函数，所以只需要考虑 $f(x)$ 的可导性。

当 $x>1$ 时，有 $f'(x)=(3x^2-1)g(x)+(x^3-x)g'(x)$。因为 $g(x)$ 连续，所以 $(3x^2-1)g(x)$ 可导，只需考虑 $(x^3-x)g'(x)$ 的可导性。因为 $x^3-x>0$，所以当 $g'(x)$ 存在时，$f(x)$ 可导。

当 $x<1$ 时，有 $f'(x)=-(3x^2-1)g(x)-(x^3-x)g'(x)$。同理可得，当 $g'(x)$ 存在时，$f(x)$ 可导。

综上，$f(x)$ 在 $x=1$ 处可导，前提是 $g'(1)$ 和 $g'(-1)$ 存在。

在 $x=-1$ 处判断：

当 $x>0$ 时，有 $f(x)=(x^3+x)g(x)$，当 $x<0$ 时，有 $f(x)=-(x^3+x)g(x)$。因为 $g(x)$ 是连续函数，所以只需要考虑 $f(x)$ 的可导性。

当 $x>0$ 时，有 $f'(x)=(3x^2+1)g(x)+(x^3+x)g'(x)$。因为 $g(x)$ 连续，所以 $(3x^2+1)g(x)$ 可导，只需考虑 $(x^3+x)g'(x)$ 的可导性。因为 $x^3+x>0$，所以当 $g'(x)$ 存在时，$f(x)$ 可导。

当 $x<0$ 时，有 $f'(x)=-(3x^2+1)g(x)-(x^3+x)g'(x)$。同理可得，当 $g'(x)$ 存在时，$f(x)$ 可导。

综上，$f(x)$ 在 $x=-1$ 处可导，前提是 $g'(1)$ 和 $g'(-1)$ 存在。

综上所述，$f(x)$ 在 $x=0$，$x=1$，$x=-1$ 处都可导，前提是 $g'(1)$ 和 $g'(-1)$ 存在。